MESI: invariants about channels

src/Ex/Mesi/MesiInv.v
@@ -15,21 +15,9 @@ Local Open Scope list.
 Local Open Scope hvec.
 Local Open Scope fmap.
 
-(* NOTE: these ltacs only work for constants (channels, objects, etc.),
- * thus will be used only in this file.
- *)
-(* Ltac get_lock_minds oidx := *)
-(*   progress (good_footprint_get oidx); *)
-(*   repeat (repeat disc_rule_conds_unit_simpl; try disc_footprints_ok); *)
-(*   disc_minds_const. *)
- 
-(* Ltac get_lock_inv obj sys := *)
-(*   let H := fresh "H" in *)
-(*   assert (In obj (sys_objs sys)) as H by (simpl; tauto); *)
-(*   progress (good_locking_get obj); *)
-(*   clear H. *)
-
 Existing Instance Mesi.ImplOStateIfc.
+
+(** Common Invariants that might be shared with the MOSI case study *)
 
 Definition MsgExistsSig (sig: MSig) (msgs: MessagePool Msg) :=
   exists idm, InMPI msgs idm /\ sigOf idm = sig.
@@ -100,12 +88,144 @@ Section ObjUnit.
     Qed.
 
   End Facts.
-  
+
 End ObjUnit.
+
+Section MsgConflicts.
+
+  Definition RsDownConflicts (oidx: IdxT) (msgs: MessagePool Msg) :=
+    forall rsDown,
+      fst (sigOf rsDown) = downTo oidx ->
+      fst (snd (sigOf rsDown)) = MRs ->
+      InMPI msgs rsDown ->
+      (forall rqUp,
+          fst (sigOf rqUp) = rqUpFrom oidx ->
+          InMPI msgs rqUp -> False) /\
+      (forall rrsDown,
+          fst (sigOf rrsDown) = downTo oidx ->
+          fst (snd (sigOf rrsDown)) = MRs ->
+          valOf rsDown <> valOf rrsDown ->
+          InMPI msgs rrsDown -> False) /\
+      (forall rsUp,
+          fst (sigOf rsUp) = rsUpFrom oidx ->
+          InMPI msgs rsUp -> False).
+
+  Variable (tr: tree) (bidx: IdxT).
+  Hypothesis (Htr: tr <> Node nil).
+  Let topo := fst (tree2Topo tr bidx).
+  Let cifc := snd (tree2Topo tr bidx).
+
+  Context `{OStateIfc}.
+  Variable (sys: System).
+  
+  Hypotheses (Hiorqs: GoodORqsInit (initsOf sys))
+             (Hrrs: RqRsSys topo sys)
+             (Hoinds: SubList (c_li_indices cifc ++ c_l1_indices cifc)
+                              (map (@obj_idx _) (sys_objs sys))).
+
+  Definition RsDownConflictsInv (st: MState) :=
+    forall oidx,
+      In oidx (c_li_indices cifc ++ c_l1_indices cifc) ->
+      RsDownConflicts oidx (bst_msgs st).
+
+  Lemma tree2Topo_non_root_RsDownConflicts_inv_ok:
+    InvReachable sys step_m RsDownConflictsInv.
+  Proof.
+    unfold InvReachable, RsDownConflictsInv; intros.
+
+    unfold cifc in H1.
+    rewrite c_li_indices_head_rootOf in H1 by assumption.
+    inv H1.
+
+    1: { (* the root case *)
+      (** TODO: need to prove an invariant about the root (main memory):
+       * no messages exist in any channel of the root, i.e., the RqUp, RsUp,
+       * and Down queues are all empty for the root.
+       *)
+      admit.
+    }
+
+    (* non-root cases *)
+    assert (exists pidx,
+               In pidx (c_li_indices cifc) /\
+               parentIdxOf topo oidx = Some pidx).
+    { apply in_app_or in H2; destruct H2.
+      { apply c_li_indices_tail_has_parent; assumption. }
+      { apply c_l1_indices_has_parent; assumption. }
+    }
+    destruct H1 as [pidx [? ?]].
+
+    pose proof (tree2Topo_TreeTopo tr bidx).
+    destruct H4; dest.
+    specialize (H4 _ _ H3); dest.
+
+    assert (exists obj, In obj (sys_objs sys) /\ obj_idx obj = oidx).
+    { apply in_app_or in H2; destruct H2.
+      { apply tl_In in H2.
+        apply SubList_app_4 in Hoinds; apply Hoinds in H2.
+        apply in_map_iff in H2; destruct H2 as [obj [? ?]]; subst.
+        exists obj; auto.
+      }
+      { apply SubList_app_5 in Hoinds; apply Hoinds in H2.
+        apply in_map_iff in H2; destruct H2 as [obj [? ?]]; subst.
+        exists obj; auto.
+      }
+    }
+    destruct H9 as [obj [? ?]]; subst.
+
+    assert (exists pobj, In pobj (sys_objs sys) /\ obj_idx pobj = pidx).
+    { apply SubList_app_4 in Hoinds; apply Hoinds in H1.
+      apply in_map_iff in H1; destruct H1 as [pobj [? ?]]; subst.
+      exists pobj; auto.
+    }
+    destruct H10 as [pobj [? ?]]; subst.
+
+    red; intros; repeat ssplit; intros.
+    - eapply rqUp_in_rsDown_in_false
+        with (obj0:= obj) (rqUp0:= rqUpFrom (obj_idx obj)) (rqum:= valOf rqUp)
+             (down:= downTo (obj_idx obj)) (rsdm:= valOf rsDown); eauto.
+      + unfold sigOf in H14; simpl in H14; red in H15; rewrite H14 in H15; assumption.
+      + unfold sigOf in H11; simpl in H11; red in H13; rewrite H11 in H13; assumption.
+    - eapply rsDown_in_rsDown_in_false
+        with (obj0:= obj) (down:= downTo (obj_idx obj))
+             (rsdm1:= valOf rsDown) (rsdm2:= valOf rrsDown); eauto.
+      + unfold sigOf in H11; simpl in H11; red in H13; rewrite H11 in H13; assumption.
+      + unfold sigOf in H14; simpl in H14; red in H17; rewrite H14 in H17; assumption.
+    - eapply rsDown_in_rsUp_in_false
+        with (cobj:= obj) (pobj0:= pobj) (rsUp0:= rsUpFrom (obj_idx obj))
+             (down:= downTo (obj_idx obj))
+             (rsdm:= valOf rsDown) (rsum:= valOf rsUp); eauto.
+      + unfold sigOf in H11; simpl in H11; red in H13; rewrite H11 in H13; assumption.
+      + unfold sigOf in H14; simpl in H14; red in H15; rewrite H14 in H15; assumption.
+  Admitted.
+
+End MsgConflicts.
+
+(** End of the common invariants -- *)
+
+Lemma mesi_RsDownConflicts:
+  forall tr (Htr: tr <> Node nil),
+    InvReachable (impl Htr) step_m (RsDownConflictsInv tr 0).
+Proof.
+  intros.
+  apply tree2Topo_non_root_RsDownConflicts_inv_ok; auto.
+  simpl; unfold mem, li, l1.
+  rewrite map_app.
+  do 2 rewrite map_trans.
+  do 2 rewrite map_id.
+  rewrite app_comm_cons.
+  rewrite <-c_li_indices_head_rootOf by assumption.
+  apply SubList_refl.
+Qed.
 
 Definition InvObjExcl0 (oidx: IdxT) (ost: OState) (msgs: MessagePool Msg) :=
   ObjExcl0 oidx ost msgs ->
   NoCohMsgs oidx msgs /\ CohRqI oidx ost msgs.
+
+Definition InvObjExcl1 (oidx: IdxT) (ost: OState) (msgs: MessagePool Msg) :=
+  (MsgExistsSig (downTo oidx, (MRs, mesiRsE)) msgs \/
+   MsgExistsSig (downTo oidx, (MRs, mesiRsM)) msgs) ->
+  ost#[implStatusIdx] = mesiI.
 
 Definition InvExcl (st: MState): Prop :=
   forall eidx,
